theories/rules/nop.v
@@ -59,11 +59,8 @@ Proof.
     rewrite (preserve_get_trans_gmap σ1).
     rewrite (preserve_get_hpool_gset σ1).
     rewrite (preserve_get_retri_gmap σ1).
-    rewrite (preserve_inv_trans_hpool_consistent σ1).
     rewrite (preserve_inv_trans_pgt_consistent σ1).
     rewrite (preserve_inv_trans_wellformed σ1).
-    rewrite (preserve_inv_pgt_mb_consistent σ1).
-    rewrite (preserve_inv_mb_wellformed σ1).
     rewrite p_upd_pc_mem.
     all: try rewrite p_upd_pc_pgt //.
     all: try rewrite p_upd_pc_trans //.
